\begin{equation}
	\dev{x}{t}=rx\left(1-\frac{x}{M}\right)-px
\end{equation}

\begin{align}
\dev{x}{t}&=rx\left(1-\frac{p}{r}-\frac{x}{M}\right) \\
\dev{x}{t}&=r\left(1-\frac{p}{r}\right)\left(1-\frac{x}{M\left(1-\frac{p}{r}\right)}\right)x
\end{align}

$\gamma=r\left(1-\frac{p}{r}\right)$, $K=M\left(1-\frac{p}{r}\right)$. With $\frac{p}{r}<1$

\begin{align}
	\dev{x}{t}&=\gamma x\left(1-\frac{x}{K}\right)\\
	x&=\frac{Kx_0}{x_0+\left(K-x_0\right)\mathrm{e}^{-\gamma t}}
\end{align}
\begin{align}
	x(t)=\frac{M\left(1-\frac{p}{r}\right)x_0}{x_0+\left(M-\frac{Mp}{r}-x_0\right)\mathrm{e}^{-\gamma t}}
\end{align}